Moved casestudy from Tsum5_HK to TStreamCase_Study

CaseStudies/TStreamCase_Study.thy
@@ -10,10 +10,10 @@ chapter {* Timed Streams *}
 
 theory TStreamCase_Study
 
-imports "../TStream" Tsum5_HK
+imports "../TStream" Tsum5_HK StreamCase_Study
 begin
 default_sort countable
-
+declare One_nat_def[simp del]
 (* Examples for weak causal functions *)
 
 (* tsTake on tstreams with only ticks *)
@@ -260,6 +260,874 @@ lemma non_mono_f2_spfw: "\<not>monofun (Rep_spfw f2_spfw)"
 apply (transfer)
 by (simp add: monofun_def f2_spfw_def)
 
+(*Definition of tsum5 and verification with sum5*)
+(*Helper like h for sum5 but over nat event streams*)
+primrec tsh :: "nat \<Rightarrow> nat \<Rightarrow> nat event stream \<Rightarrow> nat event stream" where
+"tsh 0 p ts =  \<epsilon>" |
+"tsh (Suc n) p ts = (if ts = \<epsilon> then \<epsilon> 
+                        else(if shd ts= \<surd> then (\<up>\<surd> \<bullet> (tsh n p (srt\<cdot>ts)))
+                                else (\<up>(\<M> (p + (\<M>\<inverse> (shd ts))))) \<bullet> (tsh n (p +(\<M>\<inverse> (shd ts))) (srt\<cdot> ts))))"
+
+(*Helper for tsum5 like sum5_h for sum5 but over nat event streams*)
+definition tsum5_h :: " nat \<Rightarrow> nat event stream \<rightarrow> nat event stream" where
+"tsum5_h p \<equiv> \<Lambda> ts. (\<Squnion>i. tsh i p ts)"
+
+(*Definition of sum5 over timed streams*)
+definition tsum5:: "nat tstream \<rightarrow> nat tstream" where
+"tsum5 \<equiv> (\<Lambda> ts. Abs_tstream (tsum5_h 0\<cdot>(Rep_tstream ts)))"
+
+
+
+(*\<bottom> contains no natural message *)
+lemma tsAbs_bot[simp]: "tsAbs\<cdot>\<bottom> = \<epsilon>"
+by(simp add: tsAbs_def)
+
+(*tsh of the empty stream is the empty stream*)
+lemma tsh_bot: "tsh n p \<epsilon> = \<epsilon>"
+by(induct_tac n,auto)
+
+(*tsAbs of \<surd> and a timed stream is tsAbs of the timed stream*)
+lemma AbsStsAbs_tick[simp]: "ts_well as \<Longrightarrow> tsAbs\<cdot> (Abs_tstream (\<up>(\<surd>)\<bullet>as)) = tsAbs\<cdot>(Abs_tstream as)"
+by(simp add: tsabs_insert)
+
+(*tsh returns \<surd>s immediately *)
+lemma tsh_tick: "tsh (Suc n) p ((\<up>\<surd>)\<bullet>as) = (\<up>\<surd>)\<bullet> tsh n p as"
+by(simp add: tsh_def)
+
+(*tsAbs of \<surd> timed stream is the empty stream*)
+lemma tsabs_abs_tick[simp]:"tsAbs\<cdot>(Abs_tstream (\<up>\<surd>)) = \<epsilon>"
+by(simp add: tsAbs_def)
+
+(*the vent stream with infinitely many \<surd> is well formed*)
+lemma tswellinftick: "ts_well ((\<up>\<surd>)\<infinity>)"
+by (simp add: ts_well_def)
+
+(*Implies that tsh of (\<up>\<surd>)\<infinity> equals (\<up>\<surd>)\<infinity>*)
+lemma tsum5_hsinf: "tsh (Suc n) p (sinftimes(\<up>\<surd>)) = (\<up>\<surd>) \<bullet> tsh n p (sinftimes (\<up>\<surd>))"
+by auto
+
+(*tsh i works at most with the first i elements of the input*)
+lemma contlub_tsh:
+  "\<forall>s p. tsh i p (stake i\<cdot>s) = tsh i p s"
+apply (induct_tac i, auto)
+apply (rule_tac x=s in scases)
+apply auto
+apply (metis (no_types, lifting) inject_scons stake_Suc surj_scons)
+apply (metis shd1 stake_Suc surj_scons)
+apply (metis shd1 stake_Suc surj_scons)
+apply (rule_tac x=s in scases)
+by auto
+
+(*helper for chain_tsh*)
+lemma chain_tsh_helper: "xa\<noteq>\<epsilon> \<and> shd xa \<noteq>\<surd> \<Longrightarrow> tsh (Suc n) x (xa) = \<up>(\<M> (x + (\<M>\<inverse> (shd xa)))) \<bullet> tsh n (x + (\<M>\<inverse> (shd xa))) (srt\<cdot>xa)"
+by simp
+
+(*tsh i \<sqsubseteq> tsh (Suc i)*)
+lemma chain_tsh: "chain tsh"
+apply (rule chainI)
+apply (subst fun_below_iff)+
+apply (induct_tac i, auto)
+apply(simp add: tsh_bot)+
+apply (rule monofun_cfun_arg)
+apply (erule_tac x="x" in allE)
+apply presburger
+apply (smt monofun_cfun_arg)
+apply(simp add: tsh_bot)+
+by (smt monofun_cfun_arg)+
+
+(*helper for mono_tsh*)
+lemma mono_tsh_helper: "x \<sqsubseteq> y \<and> x \<noteq> \<epsilon> \<Longrightarrow> shd x = shd y"
+using lessD by fastforce
+
+(* monotonicity of tsh *)
+lemma mono_tsh: 
+  "\<forall> x y q. x \<sqsubseteq> y \<longrightarrow> tsh n q x \<sqsubseteq> tsh n q y"
+apply (induct_tac n, auto)
+apply (drule lessD, erule disjE, simp)
+apply (erule exE)+
+apply (erule conjE)+
+apply (simp, rule monofun_cfun_arg, simp)
+using lessD apply fastforce
+using lessD apply fastforce
+using mono_tsh_helper
+proof -
+  fix na :: nat and x :: "nat event stream" and y :: "nat event stream" and q :: nat
+  assume a1: "x \<sqsubseteq> y"
+  assume a2: "x \<noteq> \<epsilon>"
+  assume "\<forall>x y. x \<sqsubseteq> y \<longrightarrow> (\<forall>q. tsh na q x \<sqsubseteq> tsh na q y)"
+  then show "\<up>(\<M> (q + (\<M>\<inverse> shd x))) \<bullet> tsh na (q + (\<M>\<inverse> shd x)) (srt\<cdot>x) \<sqsubseteq> \<up>(\<M> (q + (\<M>\<inverse> shd y))) \<bullet> tsh na (q + (\<M>\<inverse> shd y)) (srt\<cdot>y)"
+    using a2 a1 by (simp add: mono_tsh_helper monofun_cfun)
+qed
+
+(*#(tsh n p s) = min(n, #s)*)
+lemma cont_lub_tsum5_h2:
+  "\<forall>s p. stake n\<cdot> (tsh n p s) = tsh n p s "
+by(induct_tac n,auto)
+
+(* tsum5_h is a continuous function *)
+lemma cont_lub_tsum5_h: "cont (\<lambda> s. \<Squnion>i. tsh i p s)" 
+apply (rule cont2cont_lub)
+apply (rule ch2ch_fun)
+apply (rule chainI)
+apply (rule fun_belowD [of _ _ "p"])
+apply (rule chainE)
+apply (metis (no_types, lifting) chain_tsh)
+apply (rule pr_contI)
+apply (rule monofunI)
+apply (rule mono_tsh [rule_format], assumption)
+apply (rule allI)
+apply (rule_tac x="i" in exI)
+by (simp add: contlub_tsh)
+
+(*Describes the unfolding of tsum5_h if the first element of the stream is a natural message*)
+lemma tsum5_h_scons:"a\<noteq>\<surd> \<Longrightarrow> tsum5_h n \<cdot>(\<up>a\<bullet>s) = (\<up>(\<M>(n+(\<M>\<inverse> a)))) \<bullet> (tsum5_h (n+ (\<M>\<inverse> a))\<cdot>s)"  
+apply (simp add: tsum5_h_def)
+apply (subst beta_cfun, rule cont_lub_tsum5_h)+
+apply (subst contlub_cfun_arg)
+apply (rule ch2ch_fun, rule ch2ch_fun)
+apply (rule chainI)
+apply (rule fun_belowD [of _ _ "a"])
+apply (smt chain_tsh fun_belowI po_class.chain_def)
+apply (subst lub_range_shift [where j="Suc 0", THEN sym])
+apply (rule ch2ch_fun, rule ch2ch_fun)
+apply (rule chainI)
+apply (rule fun_belowD [of _ _ "a"])
+apply (smt chain_tsh fun_belowI po_class.chain_def)
+by (simp add: chain_tsh_helper)
+
+(*Describes the unfolding of tsum5_h if the first element of the stream is a \<surd>*)
+lemma tsum5_h_scons_tick:"tsum5_h n \<cdot>(\<up>\<surd>\<bullet>s) = \<up>\<surd> \<bullet> (tsum5_h n \<cdot>s)"
+apply (simp add: tsum5_h_def)
+apply (subst beta_cfun, rule cont_lub_tsum5_h)+
+apply (subst contlub_cfun_arg)
+apply (rule ch2ch_fun, rule ch2ch_fun)
+apply (rule chainI)
+apply (rule fun_belowD [of _ _ "n"])
+apply (smt chain_tsh fun_belowI po_class.chain_def)
+apply (subst lub_range_shift [where j="Suc 0", THEN sym])
+apply (rule ch2ch_fun, rule ch2ch_fun)
+apply (rule chainI)
+apply (rule fun_belowD [of _ _ "n"])
+apply (smt chain_tsh fun_belowI po_class.chain_def)
+by (simp add: chain_tsh_helper)
+
+(*Other lemma with the same meaning as tsum5_h_scons_tick*)
+lemma tsum5_h_scons_tick_2: "s=\<up>\<surd>\<bullet>as \<Longrightarrow> tsum5_h n\<cdot>s = (\<up>\<surd>)\<bullet>(tsum5_h n\<cdot> as)"
+by (simp add: tsum5_h_scons_tick)
+
+(*Other lemma with the same meaning as tsum5_h_scons*)
+lemma tsum5_h_scons_2:"shd s\<noteq>\<surd> \<and> s\<noteq>\<epsilon>\<Longrightarrow> tsum5_h n \<cdot>s = (\<up>(\<M>(n+(\<M>\<inverse> shd s)))) \<bullet> (tsum5_h (n+ (\<M>\<inverse> shd s))\<cdot>(srt\<cdot>s))"
+using tsum5_h_scons
+by (metis surj_scons)
+
+lemma tsum5_h_scons_tick_alternative:"a=\<surd> \<Longrightarrow> tsum5_h n \<cdot>(\<up>a\<bullet>s) = \<up>a \<bullet> (tsum5_h n \<cdot>s)"
+by(simp add: tsum5_h_scons_tick)
+
+(*tsum5_h of an empty stream is an empty stream*)
+lemma tsum5_empty[simp]: "tsum5_h p\<cdot>\<epsilon> = \<epsilon>"
+by (simp add: cont_lub_tsum5_h tsh_bot tsum5_h_def)
+
+(*unfolding tsum5_h with the definition*)
+lemma tsum5_h_unfold_tsh: "tsum5_h n \<cdot>input = (\<Squnion>i. tsh i n input)"
+apply (simp add:tsum5_h_def)
+by (simp add: cont_lub_tsum5_h)
+
+(*Shows that the message of a natural number of an nat event plus 0 is the nat event*)
+lemma msg_plus0[simp]:fixes a::"nat event" shows" a\<noteq>\<surd> \<Longrightarrow>\<M> (0+(\<M>\<inverse> a)) = a"
+by (metis add.left_neutral event.exhaust event.simps(4))
+
+(*shd of tsum5_h if the head is not \<surd>*)
+lemma tsum5_h_shd [simp]: "a\<noteq>\<surd> \<Longrightarrow> shd (tsum5_h n \<cdot>(\<up>a \<bullet> as)) = \<M> (n+(\<M>\<inverse> a))"
+by (simp add: tsum5_h_scons)
+
+(*shd of tsum5_h if the head is not \<surd>*)
+lemma tsum5_h_shd_2 [simp]: "shd s\<noteq>\<surd> \<and> s\<noteq>\<epsilon> \<Longrightarrow> shd (tsum5_h n \<cdot>s) = \<M> (n+(\<M>\<inverse> shd s))"
+by (simp add: tsum5_h_scons_2)
+
+(*The head of tsum5_h is the head of the input*)
+lemma tsum5_shd: "shd (tsum5_h 0\<cdot>ts) = shd ts"
+apply(cases "ts= \<epsilon>")
+apply simp
+apply(cases "shd ts= \<surd>")
+apply (metis shd1 surj_scons tsum5_h_scons_tick)
+by (metis msg_plus0 surj_scons tsum5_h_shd)
+
+(*A stream filtered by \<surd>s only contains \<surd>*)
+lemma "#({\<surd>} \<ominus> s) = Fin (Suc n) \<Longrightarrow> ({\<surd>} \<ominus> s)= (\<up>\<surd>)\<bullet>(srt\<cdot>({\<surd>} \<ominus> s))"
+by (metis Fin_02bot inject_Fin lnzero_def nat.simps(3) sfilter_resl2 singletonD slen_empty_eq surj_scons)
+
+(*#(tsum5_h s)is at least the length of s*)
+lemma tsum5_h_slen2: "#s \<le> #(tsum5_h a\<cdot>s)"
+apply (rule spec [where x = a])
+apply (rule ind [of _ s], auto)
+apply(subst lnle_def, simp del: lnle_conv)
+by (smt lnsuc_lnle_emb slen_scons tsum5_h_scons tsum5_h_scons_tick)
+
+(*The rest of tsum5_h s is tsum5_h (srt s) if the head of s is a \<surd>*)
+lemma tsum5_h_srt_tick: "shd s=\<surd> \<Longrightarrow>srt\<cdot>(tsum5_h n \<cdot>s) = tsum5_h n\<cdot> (srt\<cdot>s)"
+by (metis (no_types, lifting) inject_scons lshd_updis stream.sel_rews(2) stream.sel_rews(3) surj_scons tsum5_empty tsum5_h_scons_tick)
+
+(*Unfolding the rest of tsum5_h if the head is not a \<surd>*)
+lemma tsum5_h_srt: "shd s\<noteq>\<surd> \<Longrightarrow>srt\<cdot>(tsum5_h n \<cdot>s) = tsum5_h (n+(\<M>\<inverse> shd s))\<cdot> (srt\<cdot>s)"
+apply(cases "s=\<epsilon>")
+apply simp
+using tsum5_h_scons
+proof -
+  assume a1: "s \<noteq> \<epsilon>"
+  assume a2: "shd s \<noteq> \<surd>"
+  have f3: "\<up>(shd s) \<bullet> srt\<cdot>s = s"
+    using a1 by (metis surj_scons)
+  have "\<And>e s. updis (e::nat event) \<noteq> \<bottom> \<or> (\<epsilon>::nat event stream) = s"
+    by simp
+  then show ?thesis
+    using f3 a2 a1 by (metis lscons_conv stream.sel_rews(5) tsum5_h_scons)
+qed
+
+(*tsum5_h has the length of the input*)
+lemma tsum5_h_slen[simp]: "#(tsum5_h n\<cdot>s) = #s"
+apply (rule spec [where x = n])
+apply (rule ind [of _ s], auto)
+using tsum5_h_scons
+by (metis slen_scons tsum5_h_scons_tick)
+
+(*Unfolds tsum5_h with a \<up>(Msg m) as the input*)
+lemma [simp]: "a\<noteq>\<surd> \<Longrightarrow> tsum5_h n\<cdot>(\<up>a) = (\<up>(\<M>(n+(\<M>\<inverse> a))))"
+by (metis lscons_conv sup'_def tsum5_empty tsum5_h_scons)
+
+(*tsum5_h of a ts_well \<up>a is \<up>a*)
+lemma tsum5_h_one[simp]: "ts_well (\<up>a) \<Longrightarrow> tsum5_h n\<cdot>(\<up>a) = \<up>(a)"
+apply(cases "a\<noteq>\<surd>")
+apply (simp add: tsOneTick)
+apply auto
+apply(insert tsum5_h_scons_tick [of n \<epsilon>])
+by simp
+
+(*Length of tsAbs ts of a timedstream ts*)
+lemma tsAbs_len[simp]: "ts_well s \<Longrightarrow> #(tsAbs\<cdot>(Abs_tstream s)) = #({e. e\<noteq>\<surd>}\<ominus> s)"
+by(subst tsabs_insert, simp)
+
+(*Length of tsum5_h of a event stream without ticks is eqaul to the length of sum5 of tsAbs*)
+lemma tsum5_h_sfilter_len: "ts_well s \<Longrightarrow> #(tsum5_h n\<cdot>({e. e\<noteq>\<surd>}\<ominus>s)) = #(sum5\<cdot>(tsAbs\<cdot>(Abs_tstream s)))"
+by simp
+
+(*sum5_h unfolding when the head of the stream is 0 is the parameter concatenated to sum5_h with the rest of the stream*)
+lemma tsum5_unfold_tsum5: "tsum5_h n\<cdot>(\<up>(\<M> 0) \<bullet> s) =\<up>(\<M> (0+n)) \<bullet> tsum5_h n \<cdot>(s)"
+apply(subst tsum5_h_scons)
+apply simp
+by simp
+
+(*the (Suc nth) element of sum5_h when the head of the stream is 0 is the nth element of sum5_h with the rest stream*)
+lemma test2_tsum5_h_help: "Fin n < #s \<longrightarrow> snth (Suc n) (tsum5_h m \<cdot>(\<up>(\<M> 0) \<bullet>s)) = snth n (tsum5_h m \<cdot>s)"
+apply(induction n)
+apply(subst tsum5_unfold_tsum5)
+apply simp
+by (simp add: tsum5_unfold_tsum5)
+
+(*the (Suc nth) element of tsum5_h when the head of the stream is \<surd> is the nth element of tsum5_h with the rest stream*)
+lemma tsum5_suc_snth_tick:"Fin n < #s \<and> shd s =\<surd> \<Longrightarrow> snth (Suc n) (tsum5_h m\<cdot>s) = snth n (tsum5_h m\<cdot>(srt\<cdot>s))"
+apply(subst tsum5_h_scons_tick_2)
+apply auto
+by (metis Fin_0 less_le lnle_Fin_0 strict_slen surj_scons)
+
+(**the (Suc nth) element of tsum5_h m s when the head of the stream is not \<surd> is the nth element of tsum5_h (m + shd s)  with the rest stream**)
+lemma tsum5_suc_snth:"Fin n < #s \<and> shd s \<noteq>\<surd> \<and> s\<noteq>\<epsilon> \<Longrightarrow> snth (Suc n) (tsum5_h m\<cdot>s) = snth n (tsum5_h (m+ \<M>\<inverse> shd s)\<cdot>(srt\<cdot>s))"
+apply(subst tsum5_h_scons_2)
+by auto
+
+(*taking only \<surd>s of tsum5_h is the same as taking \<surd>s of the input*)
+lemma tsum5_ticknum_helper[simp]: "({\<surd>} \<ominus> tsum5_h n\<cdot>ts) =({\<surd>} \<ominus> ts) "
+apply(cases "ts=\<epsilon>", simp)
+apply(induction ts arbitrary: n,auto)
+proof -
+  fix u :: "nat event discr\<^sub>\<bottom>" and ts :: "nat event stream" and n:: nat
+  assume a1: "u\<noteq>\<bottom>"
+  assume a2: "(\<And>n. ts \<noteq> \<epsilon> \<Longrightarrow> {\<surd>} \<ominus> tsum5_h n\<cdot>ts = {\<surd>} \<ominus> ts)"
+  then show "{\<surd>} \<ominus> tsum5_h n\<cdot>(u && ts) = {\<surd>} \<ominus> u && ts"
+  apply(insert a1 a2)
+  apply(cases "u=updis \<surd>")
+  apply(insert lscons_conv[of \<surd> ts])
+  apply(subst tsum5_h_scons_tick_2, auto)
+  using a2 apply force
+  apply(subst tsum5_h_scons_2)
+  apply (metis stream.con_rews(2) stream.injects stream.sel_rews(5) surj_scons)
+  apply simp
+  using a2
+  by (metis (no_types, lifting) sfilter_nin singletonD stream.con_rews(2) stream.sel_rews(4) stream.sel_rews(5) surj_scons tsum5_empty)
+qed
+
+(*There are as much \<surd>s in the output as there are in the Input*)
+lemma tsum5_ticknum[simp]:"#({\<surd>} \<ominus> tsum5_h 0\<cdot>ts) =#({\<surd>} \<ominus> ts)"
+by simp
+
+(*helper for tswell_tsum5*)
+lemma tsum5_srt2input:"(\<exists>x. srt\<cdot>(tsum5_h n\<cdot>s) = tsum5_h x\<cdot>(srt\<cdot>s))"
+apply(cases "s=\<epsilon>", simp)
+apply(cases "shd s=\<surd>")
+apply(subst tsum5_h_scons_tick_2, auto)
+using surj_scons apply fastforce
+by(subst tsum5_h_scons_2, auto)
+
+(*helper for tswell_tsum5*)
+lemma tsum5_sucn_sdrop:"(\<exists>x. sdrop (Suc n)\<cdot>(tsum5_h 0\<cdot>s) = sdrop n\<cdot> (tsum5_h x\<cdot>(srt\<cdot>s)))"
+apply(subst sdrop_forw_rt)
+using tsum5_srt2input
+by metis
+
+(*helper for tswell_tsum5*)
+lemma tsum5_sdrop2input:"(\<exists>x. sdrop n\<cdot>(tsum5_h 0\<cdot>s) = tsum5_h x\<cdot>(sdrop n\<cdot>s))"
+apply(induction n arbitrary: s, auto)
+using tsum5_sucn_sdrop
+by (smt iterate_Suc lscons_conv sdrop_def stream.sel_rews(2) stream.sel_rews(5) surj_scons tsum5_empty tsum5_h_scons tsum5_h_srt_tick up_defined)
+
+(*helper for tswell_tsum5*)
+lemma tsum5_snth2input:" (\<exists>x. snth n (tsum5_h 0\<cdot>s) = shd (tsum5_h x\<cdot> (sdrop n\<cdot> s)))"
+apply(simp add: snth_def)
+using tsum5_sdrop2input by metis
+
+(*if the nth element of the input is a \<surd> so is the nth element of the output*)
+lemma tsum5_snthtick2output:" snth n s=\<surd> \<Longrightarrow> snth n (tsum5_h 0\<cdot>s) =\<surd>"
+apply(simp add: snth_def)
+apply(insert tsum5_snth2input[of n s])
+apply auto
+by (metis shd1 snth_def surj_scons tsum5_empty tsum5_h_scons_tick)
+
+(*if the input has a \<surd> at the end so does the output*)
+lemma tsum5_sfoot_helper:"#s<\<infinity> \<Longrightarrow> sfoot (tsum5_h 0\<cdot>(s \<bullet> \<up>\<surd>)) = \<surd>"
+apply(simp add: sfoot_def)
+apply(subst tsum5_snthtick2output, auto)
+by(insert sfoot12[of s \<surd>],simp add: sfoot_def)
+
+(*if the input of tsum5_h is well formed so is the output*)
+lemma tswell_tsum5:"ts_well ts \<Longrightarrow> ts_well (tsum5_h 0\<cdot>ts)"
+apply(cases "#ts=\<infinity>")
+apply(simp add: ts_well_def, auto)+
+using tsum5_sfoot_helper
+by (metis inf_ub less_le sconc_fst_inf sfoot2)
+
+(*unfolding of tsum5 with the definition*)
+lemma tsum5_unfold: "tsum5\<cdot> ts = Abs_tstream (tsum5_h 0\<cdot> (Rep_tstream ts))"
+by (simp add: tsum5_def tswell_tsum5)
+
+
+(*Test of tsum5*)
+
+(*the test nat event stream is well formed*)
+lemma tswell_test: "ts_well ((<[n1,\<surd>,n2,\<surd>,\<surd>,n3]>) \<bullet> (sinftimes(\<up>\<surd>)))"
+by(simp add: ts_well_def)
+
+(*Result of the first part of the teststream with tsum5_h 0*)
+lemma tsum5_h_test_helper1: "tsum5_h 0\<cdot>(<[\<M> 1,\<surd>,\<M> 2,\<surd>,\<surd>,\<M> 4]>) =(<[\<M> 1,\<surd>,\<M> 3,\<surd>,\<surd>,\<M> 7]>)"
+by (simp add: tsum5_h_scons tsum5_h_scons_tick numeral_3_eq_3)
+
+(*result of the last part of the teststream with tsum5_h n*)
+lemma tsum5_h_test_helper2: "tsum5_h n \<cdot>(sinftimes(\<up>\<surd>)) = sinftimes(\<up>\<surd>)"
+by (metis s2sinftimes sinftimes_unfold tsum5_h_scons_tick)
+
+(*result of the teststream with tsum5_h 0*)
+lemma tsum5_h_test: "tsum5_h 0 \<cdot>((<[\<M> 1,\<surd>,\<M> 2,\<surd>,\<surd>,\<M> 4]>) \<bullet> (sinftimes(\<up>\<surd>))) = ((<[\<M> 1,\<surd>,\<M> 3,\<surd>,\<surd>,\<M> 7]>) \<bullet> (sinftimes(\<up>\<surd>)))"
+using tsum5_h_test_helper1 tsum5_h_test_helper2
+by (simp add: tsum5_h_scons tsum5_h_scons_tick numeral_3_eq_3)
+
+(*Tests the output of tsum5*)
+lemma tssum5_test:"tsum5\<cdot> (Abs_tstream ((<[\<M> 1, \<surd>, \<M> 2, \<surd>, \<surd>, \<M> 4]>) \<bullet> (sinftimes(\<up>\<surd>))))
+ =(Abs_tstream ((<[\<M> 1,\<surd>,\<M> 3,\<surd>,\<surd>,\<M> 7]>) \<bullet> (sinftimes(\<up>\<surd>))))"
+apply(simp add: tsum5_unfold)
+apply (subst Rep_Abs)
+using tswell_test apply auto
+using tsum5_h_test_helper2
+by (simp add: tsum5_h_scons tsum5_h_scons_tick numeral_3_eq_3)
+
+
+(*tsAbs(tsum5 ts) = sum5(tsAbs ts)*)
+
+(*\<M>\<inverse> of \<M> a is a*)
+lemma[simp]:"\<M>\<inverse> (\<M> a) = a "
+by simp
+
+(*the (Suc nth) element of tsum5_h m s of a stream without \<surd>s is the nth element of tsum5_h (m+ shd s) with the rest stream*)
+lemma tsum5_sfilter_snth_helper:"Fin n < #({e. e\<noteq>\<surd>}\<ominus> s) \<and> ({e. e\<noteq>\<surd>}\<ominus> s)\<noteq>\<epsilon> \<Longrightarrow> snth (Suc n) (tsum5_h m\<cdot>({e. e\<noteq>\<surd>}\<ominus> s)) = snth n (tsum5_h (m+ \<M>\<inverse> shd ({e. e\<noteq>\<surd>}\<ominus> s))\<cdot>(srt\<cdot>({e. e\<noteq>\<surd>}\<ominus> s)))"
+apply(subst tsum5_h_scons_2)
+using sfilter_ne_resup apply auto[1]
+by auto
+
+(*sfilter_lemmas*)
+lemma sfilter_filtered: "({a} \<ominus> ({e. e \<noteq> a} \<ominus> s)) = \<epsilon>"
+using ex_snth_in_sfilter_nempty by auto
+
+lemma sfilter_length_srt: "#({a}\<ominus> (srt\<cdot>s)) \<le> #({a}\<ominus> s)"
+by (metis (no_types, lifting) eq_iff less_lnsuc sfilter_in sfilter_nin slen_scons stream.sel_rews(2) surj_scons)
+
+(*helper for tsum5_h_sfilter_snth*)
+lemma sfilter_filtered_len_srt: "({a} \<ominus> (srt\<cdot>({e. e \<noteq> a} \<ominus> s))) = \<epsilon>"
+by (metis (mono_tags, lifting) mem_Collect_eq sdom_sfilter1 sfilter2dom sfilter_srtdwl3)
+
+(*The nat of snth nat event of tsum5_h m s is the snth of tsum5_h 0 s + m*)
+lemma tsum5_sfilter_snth_unfold:"Fin n < #s \<and> #({\<surd>}\<ominus> s) = 0 \<Longrightarrow> \<M>\<inverse> snth n (tsum5_h m\<cdot>s) = \<M>\<inverse> snth n (tsum5_h 0\<cdot>s) + m"
+apply(induction n arbitrary: m s, simp)
+apply(subst tsum5_h_scons_2)
+apply (metis lnsuc_neq_0_rev sfilter_in singletonI slen_empty_eq slen_scons surj_scons)
+apply (subst tsum5_h_shd_2)
+apply (metis lnsuc_neq_0_rev sfilter_in singletonI slen_empty_eq slen_scons surj_scons)
+apply simp
+apply simp
+apply(simp add: snth_rt)
+apply(insert tsum5_h_srt, auto)
+by (smt Fin_Suc add.commute add.left_commute insert_iff less_imp_not_less lnle_Fin_0 lnsuc_lnle_emb lscons_conv not_less old.nat.distinct(2) ord_eq_less_trans sfilter_in sfilter_nin slen_empty_eq slen_scons stream.con_rews(2) surj_scons)
+
+
+(*without \<surd>s in stream tsum5_h unfolding the snth+1 element *)
+lemma tsum5_h_sfilter_snth:"Fin (Suc n) < #({e. e\<noteq>\<surd>}\<ominus> s) \<and> ({e. e\<noteq>\<surd>}\<ominus> s)\<noteq>\<epsilon> \<Longrightarrow> 
+\<M>\<inverse> snth (Suc n) (tsum5_h m\<cdot>({e. e\<noteq>\<surd>}\<ominus> s)) = \<M>\<inverse> snth n (tsum5_h 0\<cdot>(srt\<cdot>({e. e\<noteq>\<surd>}\<ominus> s))) +(m+ \<M>\<inverse> shd ({e. e\<noteq>\<surd>}\<ominus> s))"
+apply(subst tsum5_sfilter_snth_helper)
+apply simp
+apply (metis Fin_leq_Suc_leq Suc_n_not_le_n less2nat_lemma less_le)
+apply(subst tsum5_sfilter_snth_unfold)
+apply(subst sfilter_filtered_len_srt, simp)
+apply (metis Fin_Suc lnsuc_lnle_emb not_less slen_scons surj_scons)
+by simp
+
+lemma tsum5_sfilter_snth:"Fin (Suc n) < #({e. e\<noteq>\<surd>}\<ominus> s) \<and> ({e. e\<noteq>\<surd>}\<ominus> s)\<noteq>\<epsilon> \<Longrightarrow> 
+\<M>\<inverse> snth (Suc n) (tsum5_h 0\<cdot>({e. e\<noteq>\<surd>}\<ominus> s)) = \<M>\<inverse> snth n (tsum5_h 0\<cdot>(srt\<cdot>({e. e\<noteq>\<surd>}\<ominus> s))) +\<M>\<inverse> shd ({e. e\<noteq>\<surd>}\<ominus> s)"
+by(insert tsum5_h_sfilter_snth [of n s 0], simp)
+
+lemma sum3_snth_2:"Fin (Suc n) < #s \<Longrightarrow> snth (Suc n) (sum3\<cdot>s) = snth n (sum3\<cdot>(srt\<cdot>s)) + shd s"
+apply(insert sum3_snth[of n s 0], simp)
+by (metis less_le lnle_Fin_0 nat.distinct(1) not_less slen_rt_ile_eq strict_slen sum4_snth sum52sum3 sum52sum4 surj_scons)
+
+(*special case for snth 0 (smap f\<cdot>s)*)
+lemma [simp]:"s\<noteq> \<epsilon> \<Longrightarrow> shd (smap f\<cdot>s) = f (shd s)"
+apply(insert smap_snth_lemma [of 0], simp)
+by (smt shd1 smap_scons surj_scons)
+
+(*another variant of sum4_snth*)
+lemma sum4_snth_2:"Fin (Suc n) < #s \<Longrightarrow> snth (Suc n) (sum4\<cdot>s) = snth n (sum4\<cdot>(srt\<cdot>s)) + shd s"
+using sum4_snth
+by (metis less_le lnle_Fin_0 nat.distinct(1) not_less slen_rt_ile_eq strict_slen surj_scons)
+
+lemma sfilter_sfilter[simp]: "{a}\<ominus>{a}\<ominus>s = {a}\<ominus>s"
+by simp
+
+lemma tsum5_h_snth2sum3_snth:"Fin n < #({e. e\<noteq>\<surd>}\<ominus> s) \<and> ({e. e\<noteq>\<surd>}\<ominus> s)\<noteq>\<epsilon> \<Longrightarrow>
+ \<M>\<inverse> snth n (tsum5_h 0\<cdot>({e. e\<noteq>\<surd>}\<ominus> s)) = snth n (sum3\<cdot>(smap (\<lambda>e. \<M>\<inverse> e)\<cdot>({e. e\<noteq>\<surd>}\<ominus> s)))"
+apply(induction n arbitrary: s, simp+)
+apply(subst tsum5_h_shd_2, simp)
+using sfilter_ne_resup apply auto[1]
+apply simp
+apply(subst tsum5_sfilter_snth)
+apply linarith
+apply(subst sum3_snth_2)
+apply simp+
+by (smt inject_scons less2lnleD lnle_Fin_0 nat.distinct(1) not_less sfilter_srtdwl3 slen_rt_ile_eq slen_smap smap1 smap_split strict_slen surj_scons)
+
+(*helper for tsum52sum4_helper*)
+lemma tsum5_h2sum3:"smap (\<lambda>e. \<M>\<inverse> e)\<cdot> (tsum5_h 0\<cdot>({e. e\<noteq>\<surd>}\<ominus> s)) = sum3\<cdot>(smap (\<lambda>e. \<M>\<inverse> e)\<cdot>({e. e\<noteq>\<surd>}\<ominus> s))"
+apply(rule snths_eq, simp)
+apply auto
+apply(subst smap_snth_lemma)
+apply simp
+apply(rule tsum5_h_snth2sum3_snth, auto)
+by (metis Fin_0 less_le lnle_Fin_0)
+
+(*If you filter out \<surd>s the length of the input stream is equal to the length of the output stream*)
+lemma sfilter_in_tsum_helper_len[simp]: " #({e. e \<noteq> \<surd>} \<ominus> tsum5_h n\<cdot>ts) = #({e. e \<noteq> \<surd>} \<ominus> ts)"
+apply(induction ts arbitrary: n, auto)
+proof -
+  fix u :: "nat event discr\<^sub>\<bottom>" and ts :: "nat event stream" and n:: nat
+  assume a1: "u\<noteq>\<bottom>"
+  assume a2: "(\<And>n. #({e. e \<noteq> \<surd>} \<ominus> tsum5_h n\<cdot>ts) = #({e. e \<noteq> \<surd>} \<ominus> ts))"
+  then show "#({e. e \<noteq> \<surd>} \<ominus> tsum5_h n\<cdot>(u && ts)) = #({e. e \<noteq> \<surd>} \<ominus> u && ts)"
+  apply(insert a1 a2)
+  apply(cases "u=updis \<surd>")
+  apply(insert lscons_conv[of \<surd> ts])
+  apply(subst tsum5_h_scons_tick_2, auto)
+  apply(subst tsum5_h_scons_2)
+  apply (metis stream.con_rews(2) stream.injects stream.sel_rews(5) surj_scons)
+  apply simp
+by (smt lshd_updis mem_Collect_eq sfilter_in slen_scons stream.con_rews(2) stream.sel_rews(4) stream.sel_rews(5) surj_scons)
+qed
+
+(*it does not matter if i filter out the \<surd>s in at the input or the output*)
+lemma sfilter_in_tsum5:"{e. e \<noteq> \<surd>} \<ominus> tsum5_h n\<cdot>ts = tsum5_h n\<cdot>({e. e \<noteq> \<surd>} \<ominus> ts)"
+apply(cases "ts=\<epsilon>",simp)
+apply(induction ts arbitrary: n, auto)
+proof -
+  fix u :: "nat event discr\<^sub>\<bottom>" and ts :: "nat event stream" and n:: nat
+  assume a1: "u\<noteq>\<bottom>"
+  assume a2: "(\<And>n. ts \<noteq> \<epsilon> \<Longrightarrow> {e. e \<noteq> \<surd>} \<ominus> tsum5_h n\<cdot>ts = tsum5_h n\<cdot>({e. e \<noteq> \<surd>} \<ominus> ts))"
+  then show "{e. e \<noteq> \<surd>} \<ominus> tsum5_h n\<cdot>(u && ts) = tsum5_h n\<cdot>({e. e \<noteq> \<surd>} \<ominus> u && ts)"
+  apply(insert a1 a2)
+  apply(cases "u=updis \<surd>")
+  apply(insert lscons_conv[of \<surd> ts])
+  apply(subst tsum5_h_scons_tick_2, auto)
+  apply fastforce
+  apply(subst tsum5_h_scons_2)
+  apply (metis stream.con_rews(2) stream.injects stream.sel_rews(5) surj_scons)
+  apply simp
+  by (smt mem_Collect_eq sfilter_in stream.con_rews(2) stream.injects stream.sel_rews(5) strict_sfilter surj_scons tsum5_empty tsum5_h_scons)
+qed
+
+(*helper for tsum52sum4*)
+lemma tsum52sum3_helper:"smap (\<lambda>e. \<M>\<inverse> e)\<cdot> ({e. e\<noteq>\<surd>}\<ominus> (Rep_tstream (tsum5\<cdot> ts))) = sum3\<cdot>(smap (\<lambda>e. \<M>\<inverse> e)\<cdot>({e. e\<noteq>\<surd>}\<ominus> (Rep_tstream ts)))"
+apply(subst tsum5_unfold)
+apply(subst Rep_Abs)
+using tswell_tsum5 apply auto
+apply(subst sfilter_in_tsum5)
+apply(subst tsum5_h2sum3)
+by simp
+
+(*tsum5 and sum4 work the same way over naturals*)
+lemma tsum52sum3:"tsAbs\<cdot>(tsum5\<cdot> ts) = sum3\<cdot>(tsAbs\<cdot>ts)"
+apply(simp add: tsabs_insert)
+by(rule tsum52sum3_helper)
+
+(*shows that tsum5 is a weak causal*)
+lemma tsWeak2tsum5:"tsWeakCausal (\<lambda> ts. Abs_tstream (tsum5_h 0\<cdot>(Rep_tstream ts)))"
+apply(subst tsWeak2cont2)
+apply(simp add: tsTickCount_def)
+apply(subst Rep_Abs, auto)
+by(simp add: tswell_tsum5)+
+
+lemma tsWeak_tsum5:"tsWeakCausal(\<lambda> ts. tsum5\<cdot>ts)"
+by(simp add: tsum5_unfold tsWeak2tsum5)
+
+(*definition tsum_nth like sum_nth*)
+primrec tsum_nth:: "nat \<Rightarrow> nat event stream \<Rightarrow> nat" where
+"tsum_nth 0 s = (if shd s=\<surd> then 0 else \<M>\<inverse> shd s)" |
+"tsum_nth (Suc n) s = (if shd s=\<surd> then 0 + tsum_nth n (srt\<cdot>s) else (\<M>\<inverse>(shd s)) + tsum_nth n (srt\<cdot>s))"
+
+
+
+(*if the nth element of the output is a \<surd> so is the nth element of the input*)
+lemma tsum5_snthtick2input:" snth n (tsum5_h 0\<cdot>s) =\<surd> \<Longrightarrow> snth n s =\<surd>"
+by (metis event.distinct(1) shd1 snth_def surj_scons tsum5_empty tsum5_h_scons tsum5_sdrop2input)
+
+lemma tsum5_snthtick2input_equiv:" snth n (tsum5_h 0\<cdot>s) =\<surd> \<longleftrightarrow> snth n s =\<surd>"
+by(insert tsum5_snthtick2input[of n s] tsum5_snthtick2output[of n s], auto)
+
+(*if the shd s is \<surd> the sum of s is the sum of the rest of s*)
+lemma tsum_nth_suc_tick: "shd s=\<surd> \<Longrightarrow> tsum_nth (Suc n) s = tsum_nth n (srt\<cdot>s)"
+by(simp add: tsum_nth_def)
+
+(*if the shd s is not \<surd> the sum of s is the sum of the rest of s plus shd s*)
+lemma tsum_nth_suc: "shd s\<noteq>\<surd> \<Longrightarrow> tsum_nth (Suc n) s = \<M>\<inverse> shd s + tsum_nth n (srt\<cdot>s)"
+by(simp add: tsum_nth_def)
+
+(* \<M> before \<M>\<inverse>*)
+lemma MsginvMsg: "x\<noteq>\<surd> \<Longrightarrow> \<M> \<M>\<inverse>x=x"
+by (metis event.exhaust event.simps(4))
+
+(*helper for tsum5_h_2tsum_tnh_helper*)
+lemma tsum5_h_extract_state:"Fin n < #s \<and>  snth n s \<noteq> \<surd> \<and> s\<noteq>\<epsilon> \<Longrightarrow> snth n (tsum5_h m\<cdot>s) = \<M> \<M>\<inverse> snth n (tsum5_h 0\<cdot>s) + m"
+apply(induction n arbitrary: m s, auto)
+apply(simp add: snth_rt)
+proof -
+  fix s :: "nat event stream" and n:: nat and m:: nat
+  assume a1: "(\<And>m s. Fin n < #s \<and> snth n s \<noteq> \<surd> \<and> s \<noteq> \<epsilon> \<Longrightarrow> snth n (tsum5_h m\<cdot>s) = \<M> \<M>\<inverse> snth n (tsum5_h 0\<cdot>s) + m)"
+  assume a2: "Fin (Suc n) < #s"
+  assume a3: " snth n (srt\<cdot>s) \<noteq> \<surd>"
+  assume a4: "s \<noteq> \<epsilon>"
+  then show "snth n (srt\<cdot>(tsum5_h m\<cdot>s)) = \<M> \<M>\<inverse> snth n (srt\<cdot>(tsum5_h 0\<cdot>s)) + m"
+  apply(cases "shd s=\<surd>")
+  apply(simp add: tsum5_h_srt_tick)
+  apply(insert a1 a2 a3)
+  apply(metis less2lnleD lnle_Fin_0 nat.distinct(1) not_less slen_rt_ile_eq strict_slen)
+  apply(simp add: tsum5_h_srt)
+  by (smt a2 add.left_commute add.right_neutral event.inject event.simps(4) less2lnleD lnle_Fin_0 not_le old.nat.distinct(2) slen_empty_eq slen_rt_ile_eq)
+qed
+
+
+(*if the nth element of the input is not \<surd>, then the nth element of the output is equal to tsum_nth n input*)
+lemma tsum5_h2tsum_nth_helper:"Fin n < #s \<Longrightarrow> snth n s \<noteq> \<surd> \<Longrightarrow> snth n (tsum5_h 0\<cdot>s) = \<M> tsum_nth n s"
+apply(cases "s=\<epsilon>")
+apply(simp add: lnless_def MsginvMsg)
+apply(induction n arbitrary: s,auto)
+apply(subst tsum5_suc_snth_tick)
+apply(metis Fin_leq_Suc_leq less_le not_le)
+apply (metis less2lnleD lnle_Fin_0 nat.distinct(1) not_le slen_rt_ile_eq snth_rt strict_slen)
+apply(subst tsum5_h_scons_2,simp+)
+apply(subst tsum5_h_extract_state)
+apply (metis less2lnleD lnle_Fin_0 nat.simps(3) not_le slen_rt_ile_eq snth_rt strict_slen)
+apply auto
+by (metis event.simps(4) less2lnleD lnle_Fin_0 not_le old.nat.distinct(2) slen_empty_eq slen_rt_ile_eq snth_rt)
+
+
+(*helper for tsum52tsum_nth*)
+lemma tsum5_h2tsum_nth:"Fin n< #s \<Longrightarrow> snth n (tsum5_h 0\<cdot> s) = (case (snth n s) of Msg a \<Rightarrow> \<M> tsum_nth n s | \<surd> \<Rightarrow> \<surd>)"
+apply(cases "snth n s =\<surd>")
+apply(induction n arbitrary: s, simp add: tsum5_shd)
+apply(subst tsum5_snthtick2output, auto)
+apply(subst tsum5_h2tsum_nth_helper, auto)
+by (metis event.exhaust event.simps(4))
+
+(*if the nth element of the input is \<surd>, so is the nth element of the output. Otherwise it is tsum n input for the nth element*)
+lemma tsum52tsum_nth:"Fin n< #(Rep_tstream ts) \<Longrightarrow> snth n (Rep_tstream(tsum5\<cdot> ts)) = (case (snth n (Rep_tstream ts)) of Msg a \<Rightarrow> \<M> tsum_nth n (Rep_tstream ts) | \<surd> \<Rightarrow> \<surd>) "
+apply(simp add: tsum5_unfold)
+apply(subst Rep_Abs)
+using tswell_tsum5 apply simp
+by(subst tsum5_h2tsum_nth, simp+)
+
+
+lemma tsum_nth_shd:"shd s\<noteq>\<surd> \<Longrightarrow> tsum_nth 0 s = \<M>\<inverse>shd s"
+by auto
+
+lemma "({e. e\<noteq>\<surd>}\<ominus> s) \<noteq>\<epsilon> \<Longrightarrow> shd ({e. e \<noteq> \<surd>} \<ominus> s) \<noteq> \<surd>"
+using sfilter_ne_resup by auto
+
+lemma filtereps2tsAbseps:"ts_well s \<and> {e. e \<noteq> \<surd>} \<ominus> s = \<epsilon> \<Longrightarrow> tsAbs\<cdot>(Abs_tstream s) = \<epsilon>"
+by(subst tsabs_insert, simp)
+
+
+lemma tsum_nth2sum_nth_helper:" {e. e \<noteq> \<surd>} \<ominus> s \<noteq> \<epsilon> \<Longrightarrow> shd ({e. e \<noteq> \<surd>} \<ominus> s) \<noteq> \<surd>"
+using sfilter_ne_resup by auto
+
+lemma srtSmap:"srt\<cdot>(smap f\<cdot>s) = smap f\<cdot>(srt\<cdot>s)"
+by (metis sdrop_0 sdrop_forw_rt sdrop_smap)
+
+lemma tsum_nth_nth: "Fin (Suc n) <#({e. e\<noteq>\<surd>}\<ominus> s) \<longrightarrow> tsum_nth (Suc n) ({e. e\<noteq>\<surd>}\<ominus> s) = tsum_nth n ({e. e\<noteq>\<surd>}\<ominus> s) + \<M>\<inverse>snth (Suc n) ({e. e\<noteq>\<surd>}\<ominus> s)"
+apply(induction n arbitrary: s)
+apply (metis (mono_tags, lifting) mem_Collect_eq sfilterl7 snth_rt snth_shd tsum_nth.simps(1) tsum_nth.simps(2))
+using Fin_Suc lnat_po_eq_conv lnle_def lnless_def lnsuc_lnle_emb lnzero_def minimal slen_scons snth_scons strict_slen surj_scons
+by (smt add.assoc not_less sfilter_srtdwl3 tsum_nth.simps(2))
+
+lemma tsum_nth2sum_nth:"Fin  n <#({e. e\<noteq>\<surd>}\<ominus> s)\<and>({e. e\<noteq>\<surd>}\<ominus> s) \<noteq> \<epsilon> \<Longrightarrow>ts_well s \<Longrightarrow> tsum_nth n ({e. e\<noteq>\<surd>}\<ominus> s) = sum_nth n (tsAbs\<cdot>(Abs_tstream s))"
+apply(induction n)
+apply(subst tsum_nth_shd)
+using sfilter_ne_resup mem_Collect_eq apply blast
+apply(subst sum_nth.simps)
+apply(simp add: tsabs_rep_eq)
+apply(subst tsum_nth_nth, simp)
+apply(subst sum_nth_nth, simp)
+apply(simp add: tsabs_insert)
+apply(simp add: snth_rt)
+apply(subst srtSmap)
+by (smt Suc_n_not_le_n less2nat_lemma not_le slen_rt_ile_eq smap_snth_lemma trans_lnless)
+
+lemma sdrop_eps:"Fin  n \<ge> #s \<Longrightarrow> sdrop n\<cdot>s=\<epsilon>"
+apply (induction n arbitrary: s, auto)
+by (simp add: sdrop_forw_rt slen_rt_ile_eq)
+
+lemma snth_eps:"Fin  n \<ge> #s \<Longrightarrow> snth n s= shd \<epsilon>"
+apply(simp add: snth_def)
+by(subst sdrop_eps, auto)
+
+lemma tsum_nth2sum_nth_inf:"#({e. e\<noteq>\<surd>}\<ominus> s) =\<infinity> \<Longrightarrow>ts_well s \<Longrightarrow> tsum_nth n ({e. e\<noteq>\<surd>}\<ominus> s) = sum_nth n (tsAbs\<cdot>(Abs_tstream s))"
+by (metis Inf'_neq_0_rev leI notinfI3 slen_empty_eq tsum_nth2sum_nth)
+
+
+  
+primrec list2ts_alter :: "'a event list \<Rightarrow> 'a tstream"
+where
+  list2ts_alter_0:   "list2ts_alter [] = \<bottom>" |
+  list2ts_alter_Suc: "list2ts_alter (a#as) = tsLscons\<cdot> (updis a) \<cdot>(list2ts_alter as)"
+
+(*Test tsRemDups*)
+lemma "tsRemDups\<cdot>(<[Msg 1, Msg 1, Tick, Msg 1]>\<surd>) = <[Msg 1, Tick]>\<surd>"
+  apply (simp add: tsremdups_insert)
+  by (simp add: tsmlscons_lscons tsremdups_h_delayfun)
+
+(*Tests tsProjFst*)
+lemma "tsProjFst\<cdot>(<[Msg (1, 11), Msg (2, 12), Tick]>\<surd>) = <[Msg 1, Msg 2, Tick]>\<surd>"
+  apply(simp add: tsProjFst_def)
+  by (metis (mono_tags, lifting) delayfun_nbot tsmlscons_nbot tsprojfst_delayfun tsprojfst_insert 
+  tsprojfst_mlscons tsprojfst_strict up_defined)
+
+lemma "tsProjFst\<cdot>(<[Msg (1, 11), Msg (2, 12), Tick, Msg (100, 200)]>\<surd>) = <[Msg 1, Msg 2, Tick]>\<surd>"
+  apply(simp add: tsProjFst_def)
+  by (metis (mono_tags, lifting) delayfun_nbot tsmlscons_nbot tsprojfst_delayfun tsprojfst_insert 
+  tsprojfst_mlscons tsprojfst_strict up_defined)  
+
+(************************************************)
+  subsection \<open>list2ts_alter\<close>    
+(************************************************)
+(*contains list2ts_alter def and some proofs to verify list2ts and list2ts_alter*)       
+ 
+thm tslscons_bot2
+    
+    (* NIEEE: Abs_tstream (updis \<surd> && \<epsilon>) *)
+lemma "list2tsM [Msg 1, Msg 2, Tick, Msg 3, Tick, Msg 4] = s"
+  apply simp
+  oops
+
+lemma list2ts_empty [simp]: "list2ts_alter [] = \<bottom>"
+  by simp
+
+lemma list2ts_onetick: "list2ts_alter[\<surd>]= Abs_tstream (updis \<surd> && \<bottom>)"
+  by (simp add: tslscons_insert espf2tspf_def)
+
+lemma list2ts_onemsg[simp]:"a\<noteq>\<surd> \<Longrightarrow> list2ts_alter[a] =\<bottom> "
+  by simp
+
+lemma list2ts_tickfirst:"list2ts_alter (\<surd>#as) =(Abs_tstream(<[\<surd>]>)) \<bullet> list2ts_alter as"
+  apply (simp add: tslscons_insert)
+  apply (simp add: espf2tspf_def)+
+  apply (subst lscons_conv)+
+  by (simp add: tsconc_insert)
+
+lemma list2ts_nottickfirst:"a\<noteq>\<surd> \<and> as=(b # \<surd> # bs) \<Longrightarrow>list2ts_alter (a#as) =Abs_tstream (\<up>a \<bullet> Rep_tstream (list2ts_alter as))"
+  apply (simp add: tslscons_insert)
+  apply (simp add: espf2tspf_def)+
+  by (simp add: lscons_conv)
+
+lemma tstickcount_lscons1: "t\<noteq>\<surd> \<Longrightarrow> #\<surd> tsLscons\<cdot>(updis t)\<cdot>ts = #\<surd> (ts)"
+  apply (cases "ts=\<bottom>", simp)
+  apply (subst tslscons2lscons,simp)
+  apply (simp add: tslscons2lscons tstickcount_insert)
+  by (metis lscons_conv sfilter_nin singletonD)
+
+lemma tstickcount_lscons2: " #\<surd> tsLscons\<cdot>(updis \<surd>)\<cdot>ts = lnsuc\<cdot>(#\<surd> (ts))"
+  apply (cases "ts=\<bottom>", simp)
+  apply (metis DiscrTick_def delayFun_dropFirst delayfun_nbot delayfun_tslscons_bot strict_tstickcount
+  tsdropfirst_len)
+  apply (subst tslscons2lscons,simp)
+  apply (simp add: tslscons2lscons tstickcount_insert)
+  by (simp add: lscons_conv)
+
+
+lemma "#\<surd> (list2ts_alter l) \<le> #\<surd> (list2ts_alter (a#l))"
+  apply(cases "a=\<surd>",simp)
+  apply (metis DiscrTick_def delayfun_insert delayfun_tslscons less_lnsuc tstickcount_tscons)
+  by(simp add:tstickcount_lscons1)
+  
+
+lemma list2ts_nbot2[simp]:"list2ts_alter (a@[\<surd>])\<noteq>\<bottom>"
+  by (induction a, simp+)
+
+lemma list2ts_nbot1[simp]: "list2ts_alter (a@\<surd>#as)\<noteq>\<bottom>"
+  by(induction a, simp+)
+
+lemma list2ts_unfold1:"a\<noteq>\<surd> \<Longrightarrow>list2ts_alter (a # b @ [\<surd>]) =Abs_tstream (\<up>a \<bullet> Rep_tstream (list2ts_alter (b @ [\<surd>])))"
+  apply (simp add: tslscons_insert)
+  apply (simp add: espf2tspf_def)+
+  by (simp add: lscons_conv)
+
+lemma list2ts_droplist: "filter (\<lambda>e. e=\<surd>) as =[] \<Longrightarrow> list2ts_alter as = \<bottom>"
+  apply (induction as, simp)
+  apply (subgoal_tac "a\<noteq>\<surd>")
+  apply (simp add: tslscons_insert)
+  by auto
+
+lemma list2ts_unfold2:"a \<noteq> \<surd> \<Longrightarrow> list2ts_alter (a # b @ \<surd> # bs) = Abs_tstream (\<up>a \<bullet> Rep_tstream (list2ts_alter (b @ \<surd> # bs)))"
+  apply(induction bs)
+  apply(subst list2ts_unfold1,auto)
+  apply(simp add: tslscons_insert)
+  apply (simp add: espf2tspf_def)+
+  by (simp add: lscons_conv)
+
+lemma list2ts_split:"list2ts_alter (a @ \<surd> # as) = (list2ts_alter (a @ [\<surd>])) \<bullet> (list2ts_alter as)"
+  apply (induction a, simp add: tslscons_insert)
+  apply (simp add: espf2tspf_def)+
+  apply (simp add: lscons_conv tsconc_insert)
+  apply (simp add: tslscons_insert, auto)
+  by (simp add: espf2tspf_def lscons_conv tsconc_insert)+
+
+lemma list2ts_dropend:"filter (\<lambda>e. e=\<surd>) as=[] \<Longrightarrow> list2ts_alter (a @ \<surd> # as) = list2ts_alter(a @ [\<surd>])"
+  by(subst list2ts_split, simp add: list2ts_droplist)
+  
+
+lemma list2ts_lshd1 [simp]: "a\<noteq>[] \<Longrightarrow> tsLshd\<cdot>(list2ts_alter (a @ [\<surd>])) = updis (hd a)"
+  apply(induction a,simp)
+  by (metis append_Cons list.sel(1) list2ts_alter_Suc list2ts_nbot2 tslscons_lshd)
+
+lemma list2ts_lshd_tick [simp]: "tsLshd\<cdot>(list2ts_alter (\<surd> # a)) = updis \<surd>"
+  by simp
+
+lemma list2ts_srt [simp]: "t\<noteq>\<bottom> \<Longrightarrow> tsRt\<cdot>(list2ts_alter (a # as)) = list2ts_alter (as)"
+  by simp
+
+lemma list2ts_lshd [simp]: "a\<noteq>[] \<Longrightarrow> tsLshd\<cdot>(list2ts_alter (a @ \<surd> # as)) = updis (hd a)"
+  by(induction a, simp+)
+
+lemma list2ts2list2s_lscons: "list2ts_alter (a # as @ [\<surd>]) = Abs_tstream (lscons\<cdot>(updis a)\<cdot>(list2s (as@[\<surd>])))"
+  apply (induction as arbitrary: a, simp+)
+  apply (auto simp add: tslscons_insert espf2tspf_def lscons_conv)
+  apply (metis list2ts_nbot1 lscons_conv tslscons2lscons tslscons_nbot up_defined)
+  apply (subst Rep_Abs)
+  apply (auto simp add: ts_well_def)
+  apply (simp add: less_le slen_lnsuc)
+  apply (metis sconc_scons)
+  apply (subst Rep_Abs)
+  apply (auto simp add: ts_well_def)
+  apply (simp add: less_le slen_lnsuc)
+  by (metis sconc_scons)
+
+
+lemma [simp]:" #({\<surd>} \<ominus> <ls>) \<noteq> \<infinity>"
+apply (subgoal_tac "#(<ls>)\<noteq>\<infinity>")
+using sfilterl4 apply blast
+by simp
+
+lemma list2ts2list2s_well[simp]:"ts_well (list2s ls) \<Longrightarrow> Rep_tstream (list2ts_alter ls) = list2s (ls)"
+proof(induction ls)
+  case Nil
+  then show ?case
+    by simp
+next
+  case (Cons a ls)
+  then show ?case
+    apply simp 
+    by (metis Abs_Rep Rep_Abs absts2tslscons lscons_conv stream.sel_rews(5) ts_well_drop1 up_defined)
+qed
+
+lemma list2s2list2ts_well[simp]:"ts_well (list2s ls) \<Longrightarrow>  Abs_tstream (list2s ls) = list2ts_alter (ls)"
+proof(induction ls)
+  case Nil
+  then show ?case
+    by simp
+next
+  case (Cons a ls)
+  then show ?case
+    apply simp
+    by (metis Abs_Rep Rep_Abs absts2tslscons lscons_conv stream.sel_rews(5) ts_well_drop1 up_defined)
+qed
+
+(*Test*)
+lemma testlist2ts: "list2ts_alter ([\<M> True,\<M> False, \<surd>,\<M> False]) = Abs_tstream (<[Msg True,Msg False,\<surd>]>)"
+  apply (simp add: tslscons_insert)
+  apply (simp add: espf2tspf_def)+
+  apply (subst lscons_conv)+
+  by simp
+
+(*Test*)
+lemma testlist2tsM: "list2tsM ([\<M> True,\<M> False, \<surd>,\<M> False]) = tsMLscons\<cdot>(updis True)\<cdot>(tsMLscons\<cdot>(updis False)\<cdot>(delayFun\<cdot>\<bottom>))"
+  by (simp add: tslscons_insert)
+
+(*list2s*)
+lemma list2s_sfoot_ntk:"b\<noteq>\<surd> \<Longrightarrow> sfoot (<(a@[b])>) \<noteq> \<surd> "
+  apply(subst sfoot1, simp)
+  by (simp add: less_le slen_lnsuc,simp)
+  
+
+lemma tswell_list:"ls \<noteq> [] \<Longrightarrow> last ls \<noteq>\<surd> \<Longrightarrow> \<not> ts_well (list2s ls)"
+  apply (simp add: ts_well_def, auto)
+  using list2s_inj apply fastforce
+  by (metis append_butlast_last_id list2s_sfoot_ntk sfoot1)
+
+lemma list2ts_tsntimes:"ts_well (list2s as) \<Longrightarrow>tsntimes n (list2ts_alter as) = tsntimes n (Abs_tstream (list2s as))"
+  by simp
+
+
+lemma list2ts_tsinftimes2: "tsinftimes (list2ts_alter (as@[\<surd>])) = tsinftimes (Abs_tstream (list2s (as@[\<surd>])))"
+  apply (subst list2s2list2ts_well,auto)
+  apply (simp add: ts_well_def, auto)
+  by (simp add: less_le slen_lnsuc)
+  
+  
+
+(*Spezifikation tsfork*)
+
+definition tsfork_fst::"bool event stream \<Rightarrow> 'a event stream \<Rightarrow> 'a event stream" where
+"tsfork_fst \<equiv> fix\<cdot>(\<Lambda> h. (\<lambda> bs as. if (as = \<epsilon> \<or> bs=\<epsilon>) then \<epsilon> else ( if shd bs=\<surd> then (\<up>\<surd>) \<bullet> (h(srt\<cdot>bs)(srt\<cdot>as)) else
+                        (if shd bs=\<M> True then (h (srt\<cdot>bs) (srt\<cdot>as)) else (\<up>(shd as) \<bullet> (h (srt\<cdot>bs) (srt\<cdot>as)))))))"
+
+definition tsfork_snd::"bool event stream \<Rightarrow> 'a event stream \<Rightarrow> 'a event stream" where
+"tsfork_snd \<equiv> fix\<cdot>(\<Lambda> h. (\<lambda> bs as. if (as = \<epsilon> \<or> bs =\<epsilon>) then \<epsilon> else( if shd bs=\<surd> then (\<up>\<surd>) \<bullet> (h(srt\<cdot>bs)(srt\<cdot>as)) else
+                        (if shd bs=\<M> False then (h (srt\<cdot>bs) (srt\<cdot>as)) else (\<up>(shd as) \<bullet> (h (srt\<cdot>bs) (srt\<cdot>as)))))))"
+
+definition tsfork::"bool tstream \<Rightarrow> 'a tstream \<Rightarrow> 'a tstream \<times> 'a tstream" where
+"tsfork \<equiv> \<lambda> tbs tas. (Abs_tstream (tsfork_fst (Rep_tstream tbs)(Rep_tstream tas)),Abs_tstream(tsfork_snd (Rep_tstream tbs)(Rep_tstream tas)))"
+  
+  
+  
 (* Definition of tsum6 and verification with tsum5 *)
 
 (* Compute sum of previous inputs and emit it *)
